Clean/Gadgets/SHA256/Ch32.lean
@@ -41,7 +41,9 @@ set_option maxHeartbeats 800000 in
 instance elaborated : ElaboratedCircuit (F p) Inputs (fields 32) where
   main := main
   localLength _ := 32
+  output _ i0 := varFromOffset (fields 32) i0
   localLength_eq _ _ := by simp [circuit_norm, main, ch32]
+  output_eq _ _ := by dsimp only [main, ch32, circuit_norm]
   subcircuitsConsistent _ _ := by simp +arith [circuit_norm, main, ch32]
   channelsLawful := by intro x n; simp [circuit_norm, main, ch32]
 
